lib/Lib.IntVector.fsti
@@ -20,7 +20,23 @@ val reveal_vec_1: t:v_inttype -> Lemma
   (ensures vec_t t 1 == sec_int_t t)
 
 inline_for_extraction
+val vec_t_v: #t:v_inttype -> #w:width -> vec_v_t t w -> vec_t t w
+
+inline_for_extraction
 val vec_v: #t:v_inttype -> #w:width -> vec_t t w -> vec_v_t t w
+
+val lemma_of_vec_t: #t:v_inttype -> #w:width -> f:vec_t t w -> Lemma
+  (ensures vec_t_v (vec_v f) == f)
+  [SMTPat (vec_t_v #t #w (vec_v #t #w f))]
+
+val lemma_of_vec_v_t: #t:v_inttype -> #w:width -> f:vec_v_t t w -> Lemma
+  (ensures vec_v (vec_t_v f) == f)
+  [SMTPat (vec_v #t #w (vec_t_v #t #w f))]
+
+val lemma_create_index_vec_w1: #t:v_inttype -> f:vec_t t 1 -> Lemma
+  (ensures
+    (let x:uint_t t SEC = mk_int (v (index (vec_v f) 0)) in
+    create 1 x == vec_v f))
 
 val vecv_extensionality: #t:v_inttype -> #w:width -> f1:vec_t t w -> f2:vec_t t w -> Lemma
   (requires vec_v f1 == vec_v f2)
